ebpf/PrintOp.ml
@@ -39,8 +39,10 @@ let print_condition reg pp = function
       fprintf pp "%a %ss %ld" reg r1 (comparison_name c) (camlint_of_coqint n)
   | (Ccompuimm(c, n), [r1]) ->
       fprintf pp "%a %su %ld" reg r1 (comparison_name c) (camlint_of_coqint n)
-  | _ ->
-      fprintf pp "<bad condition>"
+  | (Ccomp _ , _ ) | Ccompu _ ,_ | Ccompimm _ , _ | Ccompuimm _ ,_  -> assert false
+  | (Ccompfs c | Ccompf c) , [r1;r2] -> fprintf pp "%a %sf %a" reg r1 (comparison_name c) reg r2
+  | (Cnotcompfs c | Cnotcompf c) , [r1;r2] -> fprintf pp "%a not(%sf) %a" reg r1 (comparison_name c) reg r2
+  | _ -> assert false
 
 let print_operation reg pp = function
   | Omove, [r1] -> reg pp r1
@@ -73,6 +75,46 @@ let print_operation reg pp = function
   | Oshru, [r1;r2] -> fprintf pp "%a >>u %a" reg r1 reg r2
   | Oshruimm n, [r1] -> fprintf pp "%a >>u %ld" reg r1 (camlint_of_coqint n)
   | Ocmp c, args -> print_condition reg pp (c, args)
+  | Ocast8signed, [r1] -> fprintf pp "(8s) %a" reg r1
+  | Ocast16signed, [r1] -> fprintf pp "(16s) %a" reg r1
+  | Omulhs , [r1;r2]    -> fprintf pp "mulhs(%a,%a)" reg r1 reg r2
+  | Omulhu , [r1;r2]    -> fprintf pp "mulhu(%a,%a)" reg r1 reg r2
+  | Omod , [r1;r2]    -> fprintf pp "%a mod %a)" reg r1 reg r2
+  | Omakelong, [r1;r2]   -> fprintf pp "makelong(%a,%a)" reg r1 reg r2
+  | Olowlong, [r1]       -> fprintf pp "lowlong(%a)" reg r1
+  | Ohighlong , [r1]       -> fprintf pp "highlong(%a)" reg r1
+  | Onegf     , [r1]       -> fprintf pp "negf(%a)" reg r1
+  | Oabsf     , [r1]       -> fprintf pp "absf(%a)" reg r1
+  | Oaddf     , [r1;r2]    -> fprintf pp "%a +f %a" reg r1 reg r2
+  | Osubf     , [r1;r2]    -> fprintf pp "%a -f %a" reg r1 reg r2
+  | Omulf     , [r1;r2]    -> fprintf pp "%a *f %a" reg r1 reg r2
+  | Odivf    , [r1;r2]    -> fprintf pp "%a /f %a" reg r1 reg r2
+  | Onegfs     , [r1]       -> fprintf pp "negfs(%a)" reg r1
+  | Oabsfs     , [r1]       -> fprintf pp "absfs(%a)" reg r1
+  | Oaddfs     , [r1;r2]    -> fprintf pp "%a +s %a" reg r1 reg r2
+  | Osubfs     , [r1;r2]    -> fprintf pp "%a -s %a" reg r1 reg r2
+  | Omulfs     , [r1;r2]    -> fprintf pp "%a *s %a" reg r1 reg r2
+  | Odivfs    , [r1;r2]    -> fprintf pp "%a /s %a" reg r1 reg r2
+  | Osingleoffloat , [r]   -> fprintf pp "singleoffloat(%a)" reg r
+  | Ofloatofsingle , [r]   -> fprintf pp "floatofsingle(%a)" reg r
+  | Ointoffloat, [r]   -> fprintf pp "intoffloat(%a)" reg r
+  | Ointuoffloat , [r]   -> fprintf pp "intuoffloat(%a)" reg r
+  | Ofloatofint, [r]   -> fprintf pp "floatofint(%a)" reg r
+  | Ofloatofintu , [r]   -> fprintf pp "floatofintu(%a)" reg r
+  | Ointofsingle , [r]   -> fprintf pp "intofsingle(%a)" reg r
+  | Ointuofsingle, [r]   -> fprintf pp "intuofsingle(%a)" reg r
+  | Osingleofint,  [r]   -> fprintf pp "singleofint(%a)" reg r
+  | Osingleofintu, [r]   -> fprintf pp "singleofintu(%a)" reg r
+  | Olongoffloat, [r] -> fprintf pp "longoffloat(%a)" reg r
+  | Olonguoffloat,[r] -> fprintf pp "longuoffloat(%a)" reg r
+  | Ofloatoflong, [r] -> fprintf pp "floatoflong(%a)" reg r
+  | Ofloatoflongu,[r] -> fprintf pp "floatoflongu(%a)" reg r
+  | Olongofsingle,[r] -> fprintf pp "longofsingle(%a)" reg r
+  | Olonguofsingle,[r] -> fprintf pp "longuofsingle(%a)" reg r
+  | Osingleoflong,[r] -> fprintf pp "singleofsingle(%a)" reg r
+  | Osingleoflongu,[r]-> fprintf pp "singleoflongu(%a)" reg r
+  | Ofloatconst n , [] -> fprintf pp "%F" (camlfloat_of_coqfloat n)
+  | Osingleconst n, [] -> fprintf pp "%Ff" (camlfloat_of_coqfloat32 n)
   | _ -> fprintf pp "<bad operator>"
 
 let print_addressing reg pp = function
