test/c/integr.c
@@ -1,14 +1,14 @@
 #include <stdlib.h>
 #include <stdio.h>
 
-static double square(double x)
+static int square(int x)
 {
   return x * x;
 }
 
-static double integr(double (*f)(double), double low, double high, int n)
+static int integr(int (*f)(int), int low, int high, int n)
 {
-  double h, x, s;
+  int h, x, s;
   int i;
 
   h = (high - low) / n;
@@ -17,16 +17,17 @@ static double integr(double (*f)(double), double low, double high, int n)
   return s * h;
 }
 
-double test(int n)
+int test(int n)
 {
   return integr(square, 0.0, 1.0, n);
 }
 
 int main(int argc, char ** argv)
 {
-  int n; double r;
+  int n; int r;
+  char format[] = "integr(square, 0.0, 1.0, %d) = %g\n";
   if (argc >= 2) n = atoi(argv[1]); else n = 10000000;
   r = test(n);
-  printf("integr(square, 0.0, 1.0, %d) = %g\n", n, r);
+  printf(format, n, r);
   return 0;
 }
