test/regression/krfun.c
@@ -1,6 +1,7 @@
 /* Old-style, K&R function definitions */
 
 #include <stdio.h>
+#include <stdint.h>
 
 void f(a, b, c)
      int c, a;
@@ -12,12 +13,13 @@ void f(a, b, c)
 void g(a, b, c, d, e, x)
      const unsigned char a;
      char b[64];
-     float c;
-     double d;
-     volatile int e;
+     int c;
+     uint64_t d;
+     // volatile
+     int e;
      long long x;
 {
-  printf("g(%d, \"%s\", %a, %a, %d, %lld)\n", a, b, c, d, e, x);
+  printf("g(%li, \"%s\", %a, %a, %li, %lld)\n", a, b, c, d, e, x);
 }
 
 void h(a, b, c)
@@ -30,7 +32,7 @@ void h(a, b, c)
 int main()
 {
   f(1, "Hello", 2);
-  g(257, "World", 3.141592654, 3.141592654, -34, 12345678901234567LL);
+  g(257, "World", 3141592654, 3141592654, -34, 12345678901234567LL);
   h(6, "warning!", 7);
   return 0;
 }
