test/regression/struct9.c
@@ -4,7 +4,8 @@ struct S1 {
 };
 
 struct S1 g_77 = {0x73,9};
-struct S1 * volatile g_85 = &g_77;
+struct S1 * //volatile
+g_85 = &g_77;
 struct S1 g_204 = {0xAD,0x9086};
 
 void func_1(void)
