ebpf/Machregs.v
@@ -31,7 +31,7 @@ Require Import Op.
 Inductive mreg: Type :=
   (** Allocatable integer regs *)
   | I0: mreg | I1: mreg | I2: mreg | I3: mreg | I4: mreg
-  | I5: mreg | I6: mreg | I7: mreg | I8: mreg | I9: mreg
+  | I5: mreg | I6: mreg | I7: mreg | I8: mreg (*| I9: mreg reserved for RA *)
   (** Dummy double-precision float regs *)
   | D0: mreg | D1: mreg | D2: mreg.
 
@@ -40,7 +40,7 @@ Proof. decide equality. Defined.
 Global Opaque mreg_eq.
 
 Definition all_mregs :=
-  I0 :: I1 :: I2 :: I3 :: I4 :: I5 :: I6 :: I7 :: I8 :: I9 :: D0 :: D1 :: D2 :: nil.
+  I0 :: I1 :: I2 :: I3 :: I4 :: I5 :: I6 :: I7 :: I8 :: (*I9 ::*) D0 :: D1 :: D2 :: nil.
 
 Lemma all_mregs_complete:
   forall (r: mreg), In r all_mregs.
@@ -55,6 +55,7 @@ Global Instance Finite_mreg : Finite mreg := {
   Finite_elements := all_mregs;
   Finite_elements_spec := all_mregs_complete
 }.
+
 
 Definition mreg_type (r: mreg): typ :=
   match r with
@@ -71,7 +72,7 @@ Module IndexedMreg <: INDEXED_TYPE.
   Definition index (r: mreg): positive :=
     match r with
     | I0 => 1 | I1 => 2 | I2 => 3 | I3 => 4 | I4 => 5
-    | I5 => 6 | I6 => 7 | I7 => 8 | I8 => 9 | I9 => 10
+    | I5 => 6 | I6 => 7 | I7 => 8 | I8 => 9 (*|I9 => 10*)
     | D0  => 11 | D1 => 12 | D2 => 13
     end.
 
@@ -90,7 +91,7 @@ Local Open Scope string_scope.
 
 Definition register_names :=
   ("R0", I0) :: ("R1", I1) :: ("R2", I2) :: ("R3", I3) :: ("R4", I4) ::
-  ("R5", I5) :: ("R6", I6) :: ("R7", I7) :: ("R8", I8) :: ("R9", I9) ::
+  ("R5", I5) :: ("R6", I6) :: ("R7", I7) :: ("R8", I8) :: (*("R9", I9) ::*)
   ("D0", D0) :: ("D1", D1) :: ("D2", D2) :: nil.
 
 Definition register_by_name (s: string) : option mreg :=
@@ -167,7 +168,10 @@ Definition two_address_op (op: operation) : bool :=
   | Oand | Oandimm _ | Oor | Oorimm _
   | Oxor | Oxorimm _ | Oshl | Oshlimm _
   | Oshr | Oshrimm _ | Oshru | Oshruimm _
-  | Ocmp _ => true
+  | Ocmp (Ccomp _ | Ccompu _ | Ccompimm _ _ | Ccompuimm _ _)
+  | Odivuimm _ | Omoduimm _
+  | Omulhs | Omulhu | Omod
+                        | Ocast8signed | Ocast16signed => true
   | _ => false
   end.
 
