ebpf/ValueAOp.v
@@ -30,7 +30,6 @@ Definition eval_static_condition (cond: condition) (vl: list aval): abool :=
 Definition eval_static_addressing (addr: addressing) (vl: list aval): aval :=
   match addr, vl with
   | Aindexed n, v1::nil => offset_ptr v1 n
-  | Aglobal s ofs, nil => Ptr (Gl s ofs)
   | Ainstack ofs, nil => Ptr (Stk ofs)
   | _, _ => Vbot
   end.
@@ -72,9 +71,8 @@ Definition eval_static_operation (op: operation) (vl: list aval): aval :=
   | Ocast16signed, v1 :: nil => sign_ext 16 v1
   | Omulhs, v1::v2::nil => mulhs v1 v2
   | Omulhu, v1::v2::nil => mulhu v1 v2
-  | Odiv, v1::v2::nil => divs v1 v2
   | Omod, v1::v2::nil => mods v1 v2
-  | Oshrximm n, v1::nil => shrx v1 (I n)
+(*  | Oshrximm n, v1::nil => shrx v1 (I n)*)
   | Omakelong, v1::v2::nil => longofwords v1 v2
   | Olowlong, v1::nil => loword v1
   | Ohighlong, v1::nil => hiword v1
