extraction/extraction.v
@@ -115,7 +115,8 @@ Extract Constant Compopts.thumb =>
   "fun _ -> !Clflags.option_mthumb".
 Extract Constant Compopts.debug =>
   "fun _ -> !Clflags.option_g".
-
+Extract Constant Compopts.jump_tables =>
+  "fun _ -> !Clflags.option_jump_tables".
 (* Compiler *)
 Extract Constant Compiler.print_Clight => "PrintClight.print_if".
 Extract Constant Compiler.print_Cminor => "PrintCminor.print_if".
